Finish implementation of shared interpreter and proof soundness of interpreter and sample programs

Soundness.v
@@ -40,40 +40,36 @@ Create HintDb soundness.
 Tactic Notation "pairs" := unfold gamma_pairs; simpl; split;auto; try reflexivity.
 Hint Extern 4 => pairs.
 
-Definition sound {A B A' B' : Type} 
-  `{Galois B A} `{Galois B' A'}
-  (f : B->B') (f' : A->A') :=
-  forall b a, gamma a b -> gamma (f' a) (f b).
-Hint Unfold sound.
   
 Definition sound_store (ast : abstract_store) (st : store) : Prop := 
   forall x, gamma (ast x) (st x).
 Hint Unfold sound_store.
 
-Lemma t_update_sound : forall ast st x p n,
-  sound_store ast st ->
+Lemma t_update_sound : forall (ast : abstract_store) (st : store) x p n,
+  gamma ast st ->
   gamma p n ->
-  sound_store (t_update ast x p) (t_update st x n).
+  gamma (t_update ast x p) (t_update st x n).
 Proof. 
-  intros. unfold sound_store.  intros. unfold t_update. 
-  destruct (beq_string x x0). 
+  intros. simpl. unfold gamma_store, t_update.
+  intro x'.
+  destruct (beq_string x x'). 
   - assumption.
-  - unfold sound_store in H. apply H.
+  - apply H.
 Qed.
 
 Lemma abstract_store_join_sound_left : forall ast1 ast2 st,
-  sound_store ast1 st ->
-  sound_store (abstract_store_join ast1 ast2) st.
+  gamma ast1 st ->
+  gamma (abstract_store_join ast1 ast2) st.
 Proof. 
-  unfold sound_store. intros. unfold abstract_store_join. 
+  intros. unfold abstract_store_join. 
   constructor.
 Qed.
 
 Corollary abstract_store_join_sound_right : forall ast1 ast2 st,
-  sound_store ast2 st ->
-  sound_store (abstract_store_join ast1 ast2) st.
+  gamma ast2 st ->
+  gamma (abstract_store_join ast1 ast2) st.
 Proof.
-  unfold sound_store. intros. unfold abstract_store_join. 
+  intros. unfold abstract_store_join. 
   constructor.
 Qed.
 
@@ -84,65 +80,64 @@ forall next next' f f',
 gamma f' f ->
 gamma next' next ->
 gamma (bind_state_abstract A' B' f' next') (bind_state A B f next).
-(*
 Proof.
   intros. 
-  unfold bind_state, bind_state_abstract. unfold sound. 
-  intros. apply H3 in H5.
-  simpl in H5.
-  destruct (f' a) eqn:Hfa.
-  - destruct (f b).
+  unfold bind_state, bind_state_abstract.  
+  intros ast st Hstore. apply H3 in Hstore.
+  simpl in Hstore. 
+  destruct (f' ast) eqn:Hfa.
+  - destruct (f st).
     + (* both return a value *)
       simpl. apply H4. 
-      apply H5. apply H5.
-    + (* concrete crashes *) inversion H5.
-    + (* concrete throws exception *) inversion H5.
+      apply Hstore. apply Hstore.
+    + (* concrete crashes *) inversion Hstore.
+    + (* concrete throws exception *) inversion Hstore.
   - reflexivity.
-  - destruct (f b).
-    + inversion H5.
-    + inversion H5.
-    + simpl. simpl in H5. apply H5.
-  - unfold sound in H4. destruct (f b) eqn:Hfb.
+  - destruct (f st).
+    + inversion Hstore.
+    + inversion Hstore.
+    + simpl. simpl in Hstore. apply Hstore.
+  - destruct (f st) eqn:Hfb.
     + unfold result_doorgeven. 
-      destruct (next' a0 a1) eqn:Hnext1.
-      * simpl. destruct (next a2 s) eqn:Hnext2. 
-        { split. auto. simpl in H5. destruct H5.
+      destruct (next' a a0) eqn:Hnext1.
+      * simpl. destruct (next a1 s) eqn:Hnext2. 
+        { split. auto. simpl in Hstore. destruct Hstore.
           eapply H4 in H5. rewrite Hnext1 in H5. 
           rewrite Hnext2 in H5. simpl in H5. destruct H5.
           apply H5. auto. }
-        { destruct H5. eapply H4 in H5. rewrite Hnext1 in H5. 
+        { destruct Hstore. eapply H4 in H5. rewrite Hnext1 in H5. 
           rewrite Hnext2 in H5. inversion H5. auto. }
         { auto. }
       * reflexivity.
-      * simpl. destruct (next a2 s) eqn:Hnext2.
-        { destruct H5. eapply H4 in H5. rewrite Hnext1 in H5.
+      * simpl. destruct (next a1 s) eqn:Hnext2.
+        { destruct Hstore. eapply H4 in H5. rewrite Hnext1 in H5.
           rewrite Hnext2 in H5. inversion H5. auto. }
-        { destruct H5. eapply H4 in H5. rewrite Hnext1 in H5. 
+        { destruct Hstore. eapply H4 in H5. rewrite Hnext1 in H5. 
           rewrite Hnext2 in H5. inversion H5. auto. }
         { auto. }
-      * simpl. destruct (next a2 s) eqn:Hnext2. 
-        { split. auto. destruct H5. eapply H4 in H5. rewrite Hnext1 in H5.
+      * simpl. destruct (next a1 s) eqn:Hnext2. 
+        { split. auto. destruct Hstore. eapply H4 in H5. rewrite Hnext1 in H5.
           rewrite Hnext2 in H5. destruct H5. auto. auto. }
-        { destruct H5. eapply H4 in H5. rewrite Hnext1 in H5. rewrite Hnext2 in
+        { destruct Hstore. eapply H4 in H5. rewrite Hnext1 in H5. rewrite Hnext2 in
           H5. inversion H5. auto. }
         { auto. }
-    + inversion H5. 
+    + inversion Hstore. 
     + simpl in *. 
       destruct result_doorgeven eqn:Hdoor. 
       * (* doorgeven gives result, impossible *)
         pose proof result_doorgeven_output.
-        unfold not in H6. exfalso. eapply H6. apply Hdoor. 
+        unfold not in H5. exfalso. eapply H5. apply Hdoor. 
       * (* doorgeven crashes *)
         reflexivity. 
       * (* doorgeven gives certain exception *)
-        simpl. unfold gamma_store. intro. unfold gamma_store in H5. 
+        simpl. unfold gamma_store. intro. unfold gamma_store in Hstore. 
         apply result_doorgeven_widens_store_exception in Hdoor. 
-        inversion Hdoor. eapply widen. apply H6. apply H5.
+        inversion Hdoor. eapply widen. apply H5. apply Hstore.
       * (* doorgeven gives either exception or return *)
-        simpl. unfold gamma_store. intro. unfold gamma_store in H5.
+        simpl. unfold gamma_store. intro. unfold gamma_store in Hstore.
         apply result_doorgeven_widens_store_exception_or_result in Hdoor.
-        eapply widen. inversion Hdoor. apply H6. apply H5. 
-Qed. *) Admitted.
+        eapply widen. inversion Hdoor. apply H5. apply Hstore. 
+Qed. 
 
 Hint Resolve bind_state_sound.
 
@@ -150,27 +145,24 @@ Tactic Notation "bind" := apply bind_state_sound;auto;try reflexivity.
 Hint Extern 4 => bind.
 
 Lemma sound_parity_plus :
-  sound plus parity_plus.
+  gamma parity_plus plus.
 Proof. intros ? ? ? ? ? ?.
-  unfold sound. simpl. unfold gamma_fun; intros. simpl. 
   destruct a, a0; simpl in *; try tauto;
   auto using even_even_plus, odd_plus_r, odd_plus_l, odd_even_plus.
 Qed.
 Hint Extern 5 => apply sound_parity_plus.
 
 Lemma sound_parity_mult :
-  sound mult parity_mult.
-Proof. 
-  unfold sound. simpl. unfold gamma_fun. intros. simpl.
+  gamma parity_mult mult.
+Proof. intros ? ? ? ? ? ?.
   destruct a, a0; simpl in *; try tauto; 
   auto using even_mult_l, even_mult_r, odd_mult.
 Qed.
 Hint Extern 5 => apply sound_parity_mult.
 
 Lemma sound_parity_eq :
-  sound Nat.eqb parity_eq.
-Proof.
-  unfold sound. simpl. unfold gamma_fun. intros.
+  gamma parity_eq Nat.eqb.
+Proof. intros ? ? ? ? ? ?.
   destruct a, a0; simpl in *; try tauto; unfold not; intros.
   - apply Bool.Is_true_eq_true in H1. apply Nat.eqb_eq in H1. subst.
     eauto using not_even_and_odd. 
@@ -180,53 +172,53 @@ Qed.
 Hint Extern 5 => apply sound_parity_eq.
 
 Lemma sound_ab_and :
-  sound andb and_ab.
-Proof. 
-  unfold sound. simpl. unfold gamma_fun. intros.
+  gamma and_ab andb.
+Proof. intros ? ? ? ? ? ?.
   destruct b, b0, a, a0; simpl in *; tauto.
 Qed.
 Hint Extern 5 => apply sound_ab_and.
 
 Lemma sound_ab_or :
-  sound orb or_ab.
-Proof.
-  unfold sound. simpl. unfold gamma_fun. intros.
+  gamma or_ab orb.
+Proof. intros ? ? ? ? ? ?.
   destruct b, b0, a, a0; simpl in *; tauto.
 Qed.
 Hint Extern 5 => apply sound_ab_or.
 
 Lemma sound_ab_neg :
-  sound negb neg_ab.
-Proof.
-  unfold sound. simpl. unfold gamma_fun. intros.
+  gamma neg_ab negb.
+Proof. intros ? ? ?.
   destruct b, a; simpl in *; tauto.
 Qed.
 Hint Extern 5 => apply sound_ab_neg.
 
 Lemma ensure_par_sound : 
   gamma ensure_par ensure_nat.
-Proof. (*
-  unfold sound. intros b a Hgamma.
-  simpl. unfold gamma_fun. intros ast st Hstore. simpl.
-  destruct a, b; try inversion Hgamma; pairs.
-Qed. *) Admitted.
+Proof. intros ? ? ? ? ? ?.
+  simpl. destruct a, b; simpl; tauto. 
+Qed. 
 Hint Extern 5 => apply ensure_par_sound.
 
 Lemma ensure_abool_sound :
-  sound ensure_bool ensure_abool.
-Proof.
-  unfold sound. intros b c Hgamma.
-  simpl. unfold gamma_fun. intros ast st Hstore. simpl.
-  destruct c, b; try inversion Hgamma; pairs.
+  gamma ensure_abool ensure_bool.
+Proof. intros ? ? ? ? ? ?. 
+  simpl. destruct a, b; simpl; tauto.
 Qed.
 Hint Extern 5 => apply ensure_abool_sound.
 
 Lemma pplusM_sound : gamma pplusM plusM.
 Proof.
-  intros p1 i1 ? p2 i2 ?.
-Admitted.
+  intros p1 i1 ? p2 i2 ? ? ? ?. pairs. 
+Qed.
+Hint Extern 5 => apply pplusM_sound. 
 
-Set Debug Typeclasses.
+Lemma extract_bool_sound : forall ast st x,
+  gamma ast st ->
+  gamma (extract_ab x ast) (extract_boolean x st).
+Proof.
+
+Admitted.
+Hint Extern 5 => apply extract_bool_sound.
 
 Hint Unfold gamma_fun.
 Hint Unfold gamma_store.
@@ -238,170 +230,139 @@ Proof.
   - (* (* ENum *) simpl. unfold sound. intros. unfold gamma_result. 
     unfold extract_build_val.
     destruct c; simpl. split. apply gamma_par_extract_n_n. apply H.
-    destruct b0; simpl; auto. *) admit.
+    destruct b0; simpl; auto. *) simpl. intros ? ? ?. simpl. 
+    destruct c. simpl. pairs. apply gamma_par_extract_n_n. simpl. 
+    bind. intros ? ? ?.  auto. 
   - (* EVar *) simpl. pairs. 
-  - (* EPlus *) simpl in *. apply bind_state_sound; [assumption|].
-    intros v1 av1 Hav1.
-    apply bind_state_sound; [assumption|].
-    intros v2 av2 Hav2.
-    apply bind_state_sound; [apply ensure_par_sound; assumption|].
-    intros n1 p1 Hp1.
-    apply bind_state_sound; [apply ensure_par_sound; assumption|].
-    intros n2 p2 Hp2.
-    apply bind_state_sound; [apply pplusM_sound; assumption|].
-    intros n p Hp.
-
-
- [assumption|].
-Check bind_state_sound.
-SearchAbout sound.
-    intros v.
-    apply bind_state_sound.
-    
-unfold eval_expr, eval_expr_abstract in IHa1.
-   Print eval_expr_abstract. 
-
- intros st ast H. bind. unfold sound.
-    apply IHa1. 
-    unfold shared_eval_expr.
-    simpl. 
-    unfold sound. intros n p Hgamma. simpl. unfold gamma_fun. 
-    intros ast' st'. intros Hstore. simpl. bind.
-    unfold sound. intros n' p' Hgamma'. simpl. unfold gamma_fun.
-    intros ast'' st'' Hgamma''. simpl. bind.
-    unfold sound. intros n'' p'' Hgamman''p''. simpl. unfold gamma_fun.
-    intros ast''' st''' Hgamma_store'''. bind.
-  - (* AMult *) intros st ast Hstore. simpl. 
-    bind. intros n p Hpar. simpl. unfold gamma_fun. intros ast' st' Hstore'.
-    simpl. bind.
-    unfold sound. intros n' p' Hpar'. simpl. unfold gamma_fun.
-    intros ast'' st'' Hstore''. simpl. bind.
-    unfold sound. intros. simpl. auto.
+  - (* EPlus *) simpl in *. bind. 
+    intros v1 av1 Hav1. bind.
+    intros v2 av2 Hav2. bind.
+    intros ? ? ?.  bind. 
+  - (* EMult *)
+    simpl in *. bind. 
+    intros v1 av1 Hav1. bind. 
+    intros v2 av2 Hav2. bind. 
+    intros n1 an1 Han1. bind. 
   - (* EEq *)
-    intros. simpl. bind. unfold sound. intros. simpl. unfold gamma_fun.
-    intros. simpl. bind. unfold sound. intros. simpl. unfold gamma_fun.
-    intros. simpl. bind. unfold sound. intros. simpl. unfold gamma_fun.
-    intros. simpl. bind.
+    bind. intros v1 av1 Hav1. bind. 
+    intros v2 av2 Hav2. bind.
+    intros n1 an1 Han1. bind. 
   - (* ELe *)
-    intros. simpl. bind. unfold sound. intros. simpl. unfold gamma_fun.
-    intros. simpl. bind. unfold sound. intros. simpl. unfold gamma_fun.
-    intros. simpl. bind. unfold sound. intros. simpl. unfold gamma_fun.
-    intros. simpl. bind.
+    bind. intros ? ? ?. bind. intros ? ? ?. bind. 
+    intros ? ? ?. bind. 
   - (* ENot *)
-    intros. simpl. bind. unfold sound. intros. simpl. unfold gamma_fun.
-    intros. simpl. bind.
-  - (* EAnd *)
-    intros. simpl. bind. unfold sound. intros. simpl. unfold gamma_fun.
-    intros. simpl. bind. unfold sound. intros. simpl. unfold gamma_fun.
-    intros. simpl. bind. unfold sound. intros. simpl. unfold gamma_fun.
-    intros. simpl. bind.
+    bind. intros ? ? ?. bind.
+  - (* EAnd *) bind. intros ? ? ?. bind. intros ???. bind.
+    intros ???. bind.
 Qed.
 Hint Resolve eval_expr_sound.
 
 Lemma sound_seq : forall c1 c2,
-  sound (ceval c1) (ceval_abstract c1) ->
-  sound (ceval c2) (ceval_abstract c2) ->
-  sound (ceval (c1 ;c; c2)) (ceval_abstract (c1 ;c; c2)).
+  gamma (ceval_abstract c1) (ceval c1) ->
+  gamma (ceval_abstract c2) (ceval c2) ->
+  gamma (ceval_abstract (c1 ;c; c2)) (ceval (c1 ;c; c2)).
 Proof.
-  intros c1 c2 H1 H2. unfold sound. intros. simpl. bind.
-  unfold sound. intros. simpl. unfold gamma_fun. intros.
-    unfold sound in H2. apply H2. apply H3.
+  intros c1 c2 H1 H2. bind. 
+  intros ??????. auto. 
 Qed.
-
 Hint Resolve sound_seq.
 
 Lemma sound_assignment : forall x a,
-  sound (ceval (CAss x a)) (ceval_abstract (CAss x a)).
+  gamma  (ceval_abstract (CAss x a)) (ceval (CAss x a)).
 Proof. 
-  intros. unfold sound. intros. bind.
-  simpl. unfold sound. intros. simpl. unfold gamma_fun. intros.
-  simpl. unfold gamma_pairs. simpl. split; auto.
-  unfold gamma_store. intros x'. apply t_update_sound; assumption.
+  intros. bind. 
+  intros ???. simpl. intros ???. simpl. split; auto.
+  unfold t_update. apply t_update_sound; auto.
 Qed.
-
 Hint Resolve sound_assignment.
   
 Lemma sound_if : forall b c1 c2,
-  sound (ceval c1) (ceval_abstract c1) ->
-  sound (ceval c2) (ceval_abstract c2) ->
-  sound (ceval (CIf b c1 c2)) (ceval_abstract (CIf b c1 c2)).
+  gamma (ceval_abstract c1) (ceval c1) ->
+  gamma (ceval_abstract c2) (ceval c2) ->
+  gamma (ceval_abstract (CIf b c1 c2)) (ceval (CIf b c1 c2)).
 Proof. 
-  intros e c1 c2 H1 H2. simpl. bind.
-  unfold sound. intros cv av Hgamma. simpl.
-  unfold gamma_fun. intros. bind. unfold sound. intros.
-  unfold eval_if_abstract. unfold eval_if. simpl in *. destruct a0.
-  - (* ab_true *) destruct b0. unfold gamma_fun; intros. auto. 
-    inversion H0.
-  - (* ab_false *) destruct b0. 
-    + (* true, contradiction *) simpl in *. unfold not in H0. 
-      exfalso. apply H0. reflexivity.
-    + (* false *) unfold gamma_fun;intros. apply H2. apply H3.
-  - (* ab_top *) destruct b0.
+  intros e c1 c2 H1 H2 cv av Hgamma.  simpl. 
+  unfold ceval_abstract, ceval.
+  simpl. bind. intros ??????. bind. intros ??????. 
+  unfold eval_if_abstract, eval_if. destruct a1.
+  - (* ab_true *) destruct b1.  apply H1. assumption. 
+    inversion H3.
+  - (* ab_false *) destruct b1. 
+    + (* true, contradiction *) simpl in *. unfold not in H3. 
+      exfalso. apply H3. reflexivity.
+    + (* false *) apply H2. assumption.
+  - (* ab_top *) destruct b1. 
     + (* true *)
-      assert (preorder (ceval_abstract c1) (join_op (ceval_abstract c1) (ceval_abstract c2))).
+      assert (preorder (ceval_abstract c1) (join_op (ceval_abstract c1)
+      (ceval_abstract c2))).
       apply join_upper_bound_left.
-      unfold gamma_fun; intros.
-      simpl in H3. inversion H3; subst. 
-      eapply widen. apply H5. auto.
+      inversion H5; subst. unfold ceval_abstract in H6. 
+      eapply widen. apply H6. auto.
     + (* false *) 
       assert (preorder (ceval_abstract c2) (join_op (ceval_abstract c1) (ceval_abstract c2))).
       apply join_upper_bound_right.
-      unfold gamma_fun; intros.
-      simpl in H3. inversion H3; subst.
-      eapply widen. apply H5. auto.
-  - (* ab_bottom *) inversion H0.
+      inversion H5; subst. unfold ceval_abstract in H6.
+      eapply widen. apply H6. auto.
+  - (* ab_bottom *) inversion H3.
 Qed.
-
 Hint Resolve sound_if.
 
 Lemma sound_try_catch : forall c1 c2,
-  sound (ceval c1) (ceval_abstract c1) ->
-  sound (ceval c2) (ceval_abstract c2) ->
-  sound (ceval (CTryCatch c1 c2)) (ceval_abstract (CTryCatch c1 c2)).
+  gamma (ceval_abstract c1) (ceval c1) ->
+  gamma (ceval_abstract c2) (ceval c2) ->
+  gamma (ceval_abstract (CTryCatch c1 c2)) (ceval (CTryCatch c1 c2)).
 Proof.
-  intros c1 c2 H1 H2 st ast Hstore. 
-  unfold sound in H1. apply H1 in Hstore.
-  simpl. unfold eval_catch_abstract, eval_catch.
-  destruct (ceval_abstract c1 ast) eqn:Habs1;
-  destruct (ceval c1 st) eqn:Hconc1.
-  - apply Hstore.
-  - apply Hstore.
-  - inversion Hstore.
-  - reflexivity.
-  - reflexivity.
-  - reflexivity.
-  - inversion Hstore.
-  - inversion Hstore.
-  - simpl in *. apply H2. apply Hstore.
-  - simpl. destruct (ceval_abstract c2 a); auto.
-  - inversion Hstore.
-  - simpl. simpl in Hstore. 
-    destruct (ceval_abstract c2 a) eqn:Habs2; auto.
-    simpl. destruct (ceval c2 s) eqn:Hconc2; auto. 
-    apply H2 in Hstore. rewrite Habs2 in Hstore. 
-    rewrite Hconc2 in Hstore. inversion Hstore.
+  intros c1 c2 H1 H2 ast st Hstore. 
+  pose proof Hstore.
+  apply H1 in H.
+  destruct (ceval_abstract c1) eqn:Habs1; 
+  destruct (ceval c1) eqn:Hconc1.
+  - eapply abs_trycatch_return in Habs1; rewrite Habs1. 
+    eapply trycatch_return in Hconc1; rewrite Hconc1.
+    apply H1. apply Hstore.
+  - inversion H.
+  - inversion H.
+  - eapply abs_trycatch_crash in Habs1; rewrite Habs1. reflexivity.
+  - eapply abs_trycatch_crash in Habs1; rewrite Habs1. reflexivity.
+  - eapply abs_trycatch_crash in Habs1; rewrite Habs1. reflexivity.
+  - inversion H.
+  - inversion H.
+  - eapply abs_trycatch_exception in Habs1; rewrite Habs1. 
+    eapply trycatch_exception in Hconc1; rewrite Hconc1. apply H2. apply H.
+  - eapply abs_trycatch_exceptreturn in Habs1; rewrite Habs1. 
+    pose proof Hconc1.
+    eapply trycatch_return in Hconc1; rewrite Hconc1. 
+    simpl. destruct (shared_ceval c2); auto. simpl. 
+    rewrite H0. auto.
+  - inversion H.
+  - simpl in H. 
+    eapply abs_trycatch_exceptreturn in Habs1; rewrite Habs1. simpl.
+    destruct (shared_ceval c2) eqn:Habs2; auto. simpl.
+    eapply trycatch_exception in Hconc1; rewrite Hconc1. 
+    destruct (ceval c2 s) eqn:Hconc2; auto. 
+    apply H2 in Hstore. simpl in *. apply H2 in H.
+    rewrite Hconc2 in H. 
+    unfold ceval_abstract in H. rewrite Habs2 in H.
+    inversion H.
 Qed.
-
 Hint Resolve sound_try_catch.
 
 Lemma sound_fail : 
-  sound (ceval CThrow) (ceval_abstract CThrow).
+  gamma (ceval_abstract CThrow) (ceval CThrow).
 Proof.
-  unfold sound. intros b a H. simpl. apply H.
+  intros b a H. simpl. apply H.
 Qed.
-
 Hint Resolve sound_fail.
 
 Lemma sound_skip :
-  sound (ceval SKIP) (ceval_abstract SKIP).
+  gamma (ceval_abstract SKIP) (ceval SKIP).
 Proof.
   simpl. split; auto. 
 Qed.
-
 Hint Resolve sound_skip.
 
 Theorem sound_interpreter:
-  forall c, sound (ceval c) (ceval_abstract c).
+  forall c, gamma (ceval_abstract c) (ceval c).
 Proof.
   intros. induction c; auto with soundness.
 Qed.
@@ -414,9 +375,9 @@ Definition program1 :=
   ELSE (CAss "x" (EVal (VNat 9))).
   
 Lemma sound_program1 : 
-  sound (ceval program1) (ceval_abstract program1).
+  gamma (ceval_abstract program1) (ceval program1).
 Proof.
-  unfold sound. simpl. auto.
+  simpl. auto.
 Qed.
 
 Definition program2 :=
@@ -426,10 +387,9 @@ Definition program2 :=
   ELSE (CAss "x" (EVal (VNat 20))).
 
 Lemma sound_program2 :
-  sound (ceval program2) (ceval_abstract program2).
+  gamma (ceval_abstract program2) (ceval program2).
 Proof. 
-  unfold sound. intros. simpl. 
-  auto.
+  intros. simpl. auto.
 Qed.
 
 Definition program2' :=
@@ -439,11 +399,11 @@ Definition program2' :=
   ELSE (CAss "x" (EVal (VNat 20))).
 
 Lemma sound_program2' :
-  sound (ceval program2') (ceval_abstract program2').
+  gamma (ceval_abstract program2') (ceval program2').
 Proof. 
-unfold sound. simpl. intros. split.
+simpl. intros. split.
   - auto.
-  - unfold gamma_store. intro. simpl. 
+  - intro. simpl. 
     apply t_update_sound. apply t_update_sound. apply H. 
     simpl. repeat constructor.
     simpl. repeat constructor.
@@ -453,6 +413,6 @@ Definition program3 :=
   CAss "x" (EPlus (EVal (VNat 10)) (EVal ((VBool true)))).
   
 Lemma sound_program3 :
-  sound (ceval program3) (ceval_abstract program3).
-Proof. unfold sound. simpl. reflexivity. Qed.
+  gamma (ceval_abstract program3) (ceval program3).
+Proof. simpl.  auto. Qed.
 
