AbstractInterpreter.v
@@ -27,3 +27,43 @@ Definition eval_expr_abstract (e : expr) : AbstractState avalue :=
 
 Definition ceval_abstract (c : com) : AbstractState unit :=
   shared_ceval c.
+
+
+Lemma abs_trycatch_return : forall c1 c2 ast u a,
+  ceval_abstract c1 ast = Result.returnRA unit abstract_store u a ->
+  ceval_abstract (try c1 catch c2) ast = ceval_abstract c1 ast.
+Proof.
+  intros c1 c2 ast u a Hceval. 
+  unfold ceval_abstract in *. simpl in *.
+  unfold eval_catch_abstract. rewrite Hceval.
+  reflexivity. 
+Qed.
+
+
+Lemma abs_trycatch_crash : forall c1 c2 ast,
+  ceval_abstract c1 ast = Result.crashedA unit abstract_store ->
+  ceval_abstract (try c1 catch c2) ast = Result.crashedA unit abstract_store.
+Proof.
+  intros c1 c2 ast Hceval. 
+  unfold ceval_abstract in *. simpl in *.
+  unfold eval_catch_abstract. rewrite Hceval.
+  reflexivity. 
+Qed.
+
+Lemma abs_trycatch_exception : forall c1 c2 ast ast',
+  ceval_abstract c1 ast = Result.exceptionA unit abstract_store ast' ->
+  ceval_abstract (try c1 catch c2) ast = ceval_abstract c2 ast'.
+Proof. 
+  intros c1 c2 ast ast' Hceval. unfold ceval_abstract in *. simpl in *.
+  unfold eval_catch_abstract. rewrite Hceval. reflexivity.
+Qed.
+
+Lemma abs_trycatch_exceptreturn : forall c1 c2 u ast ast',
+  ceval_abstract c1 ast = Result.exceptionOrReturn unit abstract_store u ast' ->
+  ceval_abstract (try c1 catch c2) ast = 
+    join_op (exceptionOrReturn unit abstract_store tt ast')
+            (shared_ceval c2 ast').
+Proof. 
+  intros c1 c2 u ast ast' Hceval. unfold ceval_abstract in *. simpl in *.
+  unfold eval_catch_abstract. rewrite Hceval. reflexivity.
+Qed.
