ConcreteInterpreter.v
@@ -30,3 +30,23 @@ Definition eval_expr (e : expr) : State cvalue :=
 
 Definition ceval (c : com) : State unit :=
   shared_ceval c.
+
+Lemma trycatch_return : forall c1 c2 st u st',
+  ceval c1 st = Result.returnR unit store u st' ->
+  ceval (try c1 catch c2) st = ceval c1 st.
+Proof.
+  intros c1 c2 st u st' Hceval. 
+  unfold ceval in *. simpl in *.
+  unfold eval_catch. rewrite Hceval.
+  reflexivity. 
+Qed.
+
+Lemma trycatch_exception : forall c1 c2 st st',
+  ceval c1 st = Result.exception unit store st' ->
+  ceval (try c1 catch c2) st = ceval c2 st'.
+Proof.
+  intros c1 c2 st st' Hceval. 
+  unfold ceval in *. simpl in *.
+  unfold eval_catch. rewrite Hceval.
+  reflexivity. 
+Qed.
